more

haskell/adi/Eval.hs
@@ -1,8 +1,8 @@
-{-# LANGUAGE GeneralizedNewtypeDeriving     #-}
+{-# LANGUAGE FlexibleContexts       #-}
+{-# LANGUAGE ConstraintKinds        #-}
 
 module  Eval
-    (   Eval
-    ,   runEval
+    (   Eval 
     ,   askEnv
     ,   find
     ,   alloc
@@ -11,79 +11,51 @@ module  Eval
     )   where
 
 import Env
+import Log
 import Addr
 import Heap
 import Value
 
---import Control.Monad.Except
 import Control.Monad.State
 import Control.Monad.Reader
 import Control.Monad.Writer
-import Data.Functor.Identity
 
-type Eval = EvalT Identity
+type Eval m
+    = ( MonadReader Env m
+      , MonadWriter Log m
+      , MonadState Heap m 
+      )
 
-runEval :: Eval a -> (a, [String])
-runEval = runIdentity . runEvalT newEnv newHeap
+-- Returns current environment
+askEnv :: (MonadReader Env m) => m Env
+askEnv  = ask
 
+-- Retrieves value stored in the Heap at given memory address
+find :: (MonadState Heap m) => Addr -> m Value
+find addr = findVal addr <$> get
 
-newtype EvalT m a = EvalT 
-    { unEvalT :: ReaderT Env (WriterT [String] (StateT Heap m)) a 
-    } deriving 
-        ( Functor
-        , Applicative
-        , Monad
-        , MonadReader Env
-        , MonadWriter [String]
-        , MonadState Heap
-        )
-
-runEvalT 
-    :: (Monad m) 
-    => Env
-    -> Heap 
-    -> EvalT m a 
-    -> m (a, [String])
-runEvalT env heap m  = do
-    let m1 = unEvalT m          -- ReaderT Env (WriterT [String] (StateT Heap m)) a
-    let m2 = runReaderT m1 env  -- WriterT [String] (StateT Heap m) a
-    let m3 = runWriterT m2      -- StateT Heap m (a , [String])
-    let m4 = evalStateT m3 heap -- m (a , [String])
-    m4
-
-askEnvT :: (Monad m) => EvalT m Env
-askEnvT  = ask
-
-askEnv :: Eval Env
-askEnv = askEnvT
-
-findT :: (Monad m) => Addr -> EvalT m Value
-findT addr = findVal addr <$> get
-
-find :: Addr -> Eval Value
-find = findT
-
-allocT :: (Monad m) => EvalT m Addr
-allocT = do
+-- Allocates new memory address
+alloc :: (MonadState Heap m) => m Addr
+alloc = do
     (heap,addr) <- heapAlloc <$> get
     put heap
     return addr
 
-alloc :: Eval Addr
-alloc = allocT
-
-writeT :: (Monad m) => Addr -> Value -> EvalT m ()
-writeT addr v = do
+-- Write a value at a given memory address
+write 
+    :: (MonadState Heap m, MonadWriter Log m) 
+    => Addr 
+    -> Value 
+    -> m ()
+write addr v = do
     heap <- heapWrite addr v <$> get
     put heap
     tell ["write at address " ++ show addr ++ ": " ++ show v]
 
-write :: Addr -> Value -> Eval ()
-write = writeT
-
--- run computation in a local environment
-localEnvT :: (Monad m) => Env -> EvalT m Value -> EvalT m Value
-localEnvT env ev = EvalT $ ReaderT $ const $ runReaderT (unEvalT ev) env
-
-localEnv :: Env -> Eval Value -> Eval Value
-localEnv = localEnvT
+-- Run computation in a local environment
+localEnv 
+    :: (MonadReader Env m) 
+    => Env 
+    -> m Value 
+    -> m Value
+localEnv env ev = local (const env) ev
