haskell/adi/Eval1.hs
@@ -1,0 +1,46 @@
+{-# LANGUAGE GeneralizedNewtypeDeriving     #-}
+
+module  Eval1
+    (   Eval1
+    ,   runEval
+    )   where
+
+import Env
+import Log
+import Heap
+
+import Control.Monad.State
+import Control.Monad.Reader
+import Control.Monad.Writer
+import Data.Functor.Identity
+
+type Eval1 = EvalT Identity
+
+runEval :: Eval1 a -> (a, Log)
+runEval = runIdentity . runEvalT newEnv newHeap
+
+newtype EvalT m a = EvalT 
+    { unEvalT :: ReaderT Env (WriterT Log (StateT Heap m)) a 
+    } deriving 
+        ( Functor
+        , Applicative
+        , Monad
+        , MonadReader Env
+        , MonadWriter Log
+        , MonadState Heap
+        )
+
+runEvalT 
+    :: (Monad m) 
+    => Env
+    -> Heap 
+    -> EvalT m a 
+    -> m (a, Log)
+runEvalT env heap m  = do
+    let m1 = unEvalT m          -- ReaderT Env (WriterT [String] (StateT Heap m)) a
+    let m2 = runReaderT m1 env  -- WriterT [String] (StateT Heap m) a
+    let m3 = runWriterT m2      -- StateT Heap m (a , [String])
+    let m4 = evalStateT m3 heap -- m (a , [String])
+    m4
+
+
