haskell/adi/Log.hs
@@ -1,0 +1,6 @@
+module  Log
+    (   Log
+    )   where
+
+
+type Log = [String]
