coq/Logic/Lang1/Replacement.v
@@ -2,20 +2,51 @@ Require Import List.
 
 Require Import Logic.Axiom.LEM.
 
+Require Import Logic.Func.Replace.
+Require Import Logic.Func.Composition.
+
+Require Import Logic.Fol.Valid.
 Require Import Logic.Fol.Syntax.
+Require Import Logic.Fol.Functor.
 
 Require Import Logic.Set.Set.
 Require Import Logic.Set.Elem.
 Require Import Logic.Set.Incl.
 Require Import Logic.Set.Equal.
+Require Import Logic.Set.Functional.
 Require Import Logic.Set.Compatible.
 
+Require Import Logic.Lang1.Apply.
 Require Import Logic.Lang1.Syntax.
 Require Import Logic.Lang1.Semantics.
 Require Import Logic.Lang1.Relevance.
 Require Import Logic.Lang1.Environment.
+Require Import Logic.Lang1.Substitution.
 
-Definition replacementF (P:Formula) (n m p q:nat) : Formula :=
-    (Imp 
-        (Elem n n) (* TODO *)
-        (All n (Exi m (All p (Iff (Elem p m) (Exi q (And (Elem q n) P))))))).
+(* A n (A m (A m' (P n m -> P n m' -> m = m')))                                 *)
+Definition functionalF (P:Formula) (n m m':nat) : Formula :=
+    All n (All m (All m' (Imp (apply2 P n m) (Imp (apply2 P n m') (Equ m m'))))). 
+
+(*
+Lemma evalFunctionalF : LEM -> forall (e:Env) (P:Formula) (n m m':nat),
+    valid (replace2 0 1 n m)  P ->
+    valid (replace2 0 1 n m') P ->
+    eval e (functionalF P n m m')
+        <->
+    functional (eval2 e P 0 1).
+Proof.
+    intros L e P n m m' H1 H2. 
+    unfold functional, functionalF, apply2, eval2. rewrite evalAll.
+    split; intros H3 x.
+    - intros y y' H4 H5. 
+    remember (H3 x)  as H6 eqn:E. clear E H3. rewrite evalAll in H6.
+    remember (H6 y)  as H3 eqn:E. clear E H6. rewrite evalAll in H3.
+    remember (H3 y') as H6 eqn:E. clear E H3. rewrite evalImp in H6.
+    rewrite evalImp in H6. rewrite evalEqu in H6.
+    rewrite bindDiff in H6. rewrite bindSame in H6. rewrite bindSame in H6.
+    apply H6.
+        + apply Substitution.
+            { exact H1.     (* <- H1 *) }
+            { 
+Show.
+*)
