lean/while/ReducePar.lean
@@ -1,0 +1,15 @@
+import Stmt
+import Reduce
+
+open list
+open Stmt
+
+inductive ReducePar : list Stmt → Env → list Stmt → Env → Prop
+| Step : ∀ (e₁ e₂:Stmt) (s₁ s₂:Env) (es : list Stmt),
+    Reduce e₁ s₁ e₂ s₂ → ReducePar (e₁ :: es) s₁ (e₂ :: es) s₂
+| Cons : ∀ (es₁ es₂:list Stmt) (s₁ s₂:Env) (e:Stmt),
+    ReducePar es₁ s₁ es₂ s₂ → ReducePar (e :: es₁) s₁ (e :: es₂) s₂
+
+def p₀ : Stmt := "x" :== aNum 42
+def p₁ : Stmt := "x" :== aNum 99
+
